Working on Tailcall

backend/Tailcallproof.v
@@ -15,6 +15,7 @@
 Require Import Coqlib Maps Integers AST Linking.
 Require Import Values Memory Events Globalenvs Smallstep.
 Require Import Op Registers RTL Conventions Tailcall.
+(*SACC:*)
 Require Import StackInj.
 
 (** * Syntactic properties of the code transformation *)
@@ -211,23 +212,22 @@ Proof.
   intros. apply match_transform_program; auto.
 Qed.
 
-Section PRESERVATION.
-Context `{external_calls_prf: ExternalCalls}.
-
-Existing Instance inject_perm_all.
-
-Variable prog tprog: program.
-Hypothesis TRANSL: match_prog prog tprog.
-
+(*SACC:*)
 Definition regs_inject (j: meminj) (rs1 rs2: Regmap.t val) :=
   forall r,
     Val.inject j (rs1 # r) (rs2 # r).
 
+(*SACC:*)
 Definition inject_globals  {F V} (g: Genv.t F V) j:=
   (forall b,
       Plt b (Genv.genv_next g) -> j b = Some (b,0)) /\
   (forall b1 b2 delta,
       j b1 = Some (b2, delta) -> Plt b2 (Genv.genv_next g) -> b2 = b1 /\ delta = 0).
+
+Section PRESERVATION.
+
+Variable prog tprog: program.
+Hypothesis TRANSL: match_prog prog tprog.
 
 Let ge := Genv.globalenv prog.
 Let tge := Genv.globalenv tprog.
@@ -252,12 +252,6 @@ Lemma senv_preserved:
   Senv.equiv ge tge.
 Proof (Genv.senv_transf TRANSL).
 
-Lemma genv_next_preserved:
-  Genv.genv_next tge = Genv.genv_next ge.
-Proof.
-  apply senv_preserved.
-Qed.
-
 Lemma sig_preserved:
   forall f, funsig (transf_fundef f) = funsig f.
 Proof.
@@ -273,10 +267,11 @@ Proof.
 Qed.
 
 Lemma find_function_translated:
-  forall ros rs rs' f j,
+  forall ros rs rs' f (*SACC:*)j,
   find_function ge ros rs = Some f ->
-  regs_inject j rs rs' ->
-  inject_globals ge j ->
+  (*SACC:commented this*)(*regs_lessdef rs rs' ->*)
+  (*SACC:*)regs_inject j rs rs' ->
+  (*SACC:*)inject_globals ge j ->
   find_function tge ros rs' = Some (transf_fundef f).
 Proof.
   intros ros rs rs' f j FF RI IG; destruct ros; simpl in *.
@@ -331,57 +326,26 @@ We first define the simulation invariant between call stacks.
 The first two cases are standard, but the third case corresponds
 to a frame that was eliminated by the transformation. *)
 
-
-(**
- *
- *)
-
-Inductive match_stackframes: meminj -> nat -> list nat -> list stackframe -> list stackframe -> Prop :=
-  | match_stackframes_nil j:
-      match_stackframes j O nil nil nil
-  | match_stackframes_normal: forall j n l stk stk' res sp sp' pc rs rs' f,
-      match_stackframes j n l stk stk' ->
-      regs_inject j rs rs' ->
-      j sp = Some (sp',0) ->
-      match_stackframes j O (S n::l)
+Inductive match_stackframes: (*SACC:*)meminj -> (*SACC:*)nat -> (*SACC:*)list nat -> list stackframe -> list stackframe -> Prop :=
+  | match_stackframes_nil (*SACC:*)j:
+      match_stackframes (*SACC:*)j (*SACC:*)0 (*SACC:*)nil nil nil
+  | match_stackframes_normal: forall (*SACC:*)j (*SACC:*)n (*SACC:*)l stk stk' res sp (*SACC:*)sp' pc rs rs' f,
+      match_stackframes (*SACC:*)j (*SACC:*)n (*SACC:*)l stk stk' ->
+  (*SACC:comments this*)(*regs_lessdef rs rs' ->*)
+  (*SACC:*)regs_inject j rs rs' ->
+  (*SACC:*)j sp = Some (sp',0) ->
+      match_stackframes (*SACC:*)j (*SACC:*)0 (*SACC:*)(S n :: l)
         (Stackframe res f (Vptr sp Ptrofs.zero) pc rs :: stk)
-        (Stackframe res (transf_function f) (Vptr sp' Ptrofs.zero) pc rs' :: stk')
-  | match_stackframes_tail: forall j n l stk stk' res sp pc rs f,
-      match_stackframes j n l stk stk' ->
+        (Stackframe res (transf_function f) (Vptr (*SACC:*)sp' Ptrofs.zero) pc rs' :: stk')
+  | match_stackframes_tail: forall (*SACC:*)j (*SACC:*)n (*SACC:*)l stk stk' res sp pc rs f,
+      match_stackframes (*SACC:*)j (*SACC:*)n (*SACC:*)l stk stk' ->
       is_return_spec f pc res ->
       f.(fn_stacksize) = 0 ->
-      match_stackframes j
-                        (S n) l
-                        (Stackframe res f (Vptr sp Ptrofs.zero) pc rs :: stk)
-                        stk'.
+      match_stackframes (*SACC:*)j (*SACC:*)(S n) l
+        (Stackframe res f (Vptr sp Ptrofs.zero) pc rs :: stk)
+        stk'.
 
-
-(** Here is the invariant relating two states.  The first three
-  cases are standard.  Note the ``less defined than'' conditions
-  over values and register states, and the corresponding ``extends''
-  relation over memory states. *)
-
-Lemma sizes_upstar:
-  forall n g s1 s2 l,
-    sizes (n :: g) s1 s2 ->
-    sizes (S n :: g) ((None,l) :: s1) s2.
-Proof.
-  intros n g s1 s2 l SZ.
-  inv SZ. simpl in *. repeat destr_in H2.
-  econstructor; simpl; auto. rewrite Heqo. eauto. right; auto.
-Qed.
-
-Lemma sizes_upstar':
-  forall n g s1 s2 f l,
-    sizes (n :: g) s1 (f::s2) ->
-    sizes (S n :: g) ((None,l) :: s1) ((None,opt_cons (fst f) (snd f))::s2).
-Proof.
-  intros n g s1 s2 f l SZ.
-  inv SZ. simpl in *. repeat destr_in H5.
-  econstructor; simpl; auto. rewrite Heqo. eauto. right; auto.
-  rewrite size_frames_tc. auto.
-Qed.
-
+(*SACC:*)
 Lemma sizes_up:
   forall g s1 s2,
     sizes g s1 s2 ->
@@ -391,6 +355,7 @@ Proof.
   left. omega.
 Qed.
 
+(*SACC:*)
 Lemma sizes_record:
   forall g tf1 r1 tf2 r2 fr1 fr2 
     (SZ: sizes g (tf1 :: r1) (tf2 :: r2))
@@ -418,28 +383,28 @@ Proof.
   rewrite map_opt_cons, <- max_opt_size_frame_tailcall. auto.
 Qed.
 
+(*SACC:*)
 Definition tc_sizes: frameinj -> stack -> stack -> Prop := sizes.
 
-Definition tc_sizes_upstar:
-  forall n g s1 s2 l,
-    tc_sizes (n :: g) s1 s2 ->
-    tc_sizes (S n :: g) ((None,l) :: s1) s2 := sizes_upstar.
-
+(*SACC:*)
 Definition tc_sizes_up:
   forall g s1 s2,
     tc_sizes g s1 s2 ->
     tc_sizes (1%nat :: g) ((None,nil) :: s1) ((None,nil) :: s2) := sizes_up.
 
+(*SACC:*)
 Definition tc_sizes_ndown:
   forall n g s1 s2,
     tc_sizes (S n :: g) s1 s2 ->
     tc_sizes g (drop (S n) s1) (tl s2) := compat_sizes_drop.
 
+(*SACC:*)
 Definition tc_sizes_size_stack:
   forall g s1 s2,
     tc_sizes g s1 s2 ->
     size_stack s2 <= size_stack s1 := sizes_size_stack.
 
+(*SACC:*)
 Definition tc_sizes_record:
   forall g tf1 r1 tf2 r2 fr1 fr2 
     (SZ: tc_sizes g (tf1 :: r1) (tf2 :: r2))
@@ -447,102 +412,72 @@ Definition tc_sizes_record:
     tc_sizes g ((Some fr1, opt_cons (fst tf1) (snd tf1)) :: r1)
              ((Some fr2, opt_cons (fst tf2) (snd tf2)) :: r2) := sizes_record.
 
+(*SACC:*)
+Section STACK_WRAPPER.
+
+(*SACC:*)
 Variable fn_stack_requirements: ident -> Z.
 
-Section WITHINITMEM.
-Variable init_m: mem.
+(** Here is the invariant relating two states.  The first three
+  cases are standard.  Note the ``less defined than'' conditions
+  over values and register states, and the corresponding ``extends''
+  relation over memory states. *)
 
 Inductive match_states: state -> state -> Prop :=
   | match_states_normal:
-      forall s sp sp' pc rs m s' rs' m' f g j n l
-             (STACKS: match_stackframes j n g s s')
-             (RLD: regs_inject j rs rs')
-             (MLD: Mem.inject j (S n :: g ++ l) m m')
-             (SZ: tc_sizes (S n :: g ++ l) (Mem.stack m) (Mem.stack m'))
-             (IG: inject_globals ge j)
-             (JB: j sp = Some (sp', 0))
-             (INCR: inject_incr (Mem.flat_inj (Mem.nextblock init_m)) j)
-             (SEP: inject_separated (Mem.flat_inj (Mem.nextblock init_m)) j init_m init_m),
+      forall s sp (*SACC:*)sp' pc rs m s' rs' m' f (*SACC:*)g (*SACC:*)j (*SACC:*)n (*SACC:*)l
+             (STACKS: match_stackframes (*SACC:*)j (*SACC:*)n (*SACC:*)g s s')
+    (*SACC:comments this*)(*(RLD: regs_lessdef rs rs')*)
+    (*SACC:comments this*)(*(MLD: Mem.extends m m'),*)
+    (*SACC:*)(MLD: Mem.inject j (S n :: g ++ l) m m')
+    (*SACC:*)(SZ: tc_sizes (S n :: g ++ l) (Mem.stack m) (Mem.stack m'))
+    (*SACC:*)(IG: inject_globals ge j)
+    (*SACC:*)(JB: j sp = Some (sp', 0))
+    (*SACC:*)(*(INCR: inject_incr (Mem.flat_inj (Mem.nextblock init_m)) j)*)
+    (*SACC:*)(*(SEP: inject_separated (Mem.flat_inj (Mem.nextblock init_m)) j init_m init_m)*),
       match_states (State s f (Vptr sp Ptrofs.zero) pc rs m)
-                   (State s' (transf_function f) (Vptr sp' Ptrofs.zero) pc rs' m')
+                   (State s' (transf_function f) (Vptr (*SACC:*)sp' Ptrofs.zero) pc rs' m')
   | match_states_call:
-      forall s f args m s' args' m' sz g j n l
-        (MS: match_stackframes j n g s s')
-        (LDargs: Val.inject_list j args args')
-        (MLD: Mem.inject j (S n :: g ++ l) m m')
-        (SZ: tc_sizes (S n :: g ++ l) (Mem.stack m) (Mem.stack m'))
-        (IG: inject_globals ge j)
-        (INCR: inject_incr (Mem.flat_inj (Mem.nextblock init_m)) j)
-        (SEP: inject_separated (Mem.flat_inj (Mem.nextblock init_m)) j init_m init_m),
-      match_states (Callstate s f args m sz)
-                   (Callstate s' (transf_fundef f) args' m' sz)
+      forall s f args m s' args' m' (*SACC:*)sz (*SACC:*)g (*SACC:*)j (*SACC:*)n (*SACC:*)l
+      (MS: match_stackframes (*SACC:*)j (*SACC:*)n (*SACC:*)g s s')
+      (*SACC:comments this*)(*Val.lessdef_list args args' ->*)
+      (*SACC:comments this*)(*Mem.extends m m' ->*)
+  (*SACC:*)(LDargs: Val.inject_list j args args')
+  (*SACC:*)(MLD: Mem.inject j (S n :: g ++ l) m m')
+  (*SACC:*)(SZ: tc_sizes (S n :: g ++ l) (Mem.stack m) (Mem.stack m'))
+  (*SACC:*)(IG: inject_globals ge j)
+  (*SACC:*)(*(INCR: inject_incr (Mem.flat_inj (Mem.nextblock init_m)) j)*)
+  (*SACC:*)(*(SEP: inject_separated (Mem.flat_inj (Mem.nextblock init_m)) j init_m init_m)*),
+      match_states (Callstate s f args m (*SACC:*)sz)
+                   (Callstate s' (transf_fundef f) args' m' (*SACC:*)sz)
   | match_states_return:
-      forall s v m s' v' m' g j n l
-        (MS: match_stackframes j n g s s')
-        (LDret: Val.inject j v v')
-        (MLD: Mem.inject j (S n :: g ++ l) m m')
-        (SZ: tc_sizes (g ++ l) (drop (S n) (Mem.stack m)) (tl (Mem.stack m')))
-        (IG: inject_globals ge j)
-        (INCR: inject_incr (Mem.flat_inj (Mem.nextblock init_m)) j)
-        (SEP: inject_separated (Mem.flat_inj (Mem.nextblock init_m)) j init_m init_m),
-        match_states (Returnstate s v m)
-                     (Returnstate s' v' m')
+      forall s v m s' v' m' (*SACC:*)g (*SACC:*)j (*SACC:*)n (*SACC:*)l
+      (MS: match_stackframes (*SACC:*)j (*SACC:*)n (*SACC:*)g s s')
+      (*SACC:comments this*)(*Val.lessdef v v' ->*)
+      (*SACC:comments this*)(*Mem.extends m m' ->*)
+   (*SACC:*)(LDret: Val.inject j v v')
+   (*SACC:*)(MLD: Mem.inject j (S n :: g ++ l) m m')
+   (*SACC:*)(SZ: tc_sizes (g ++ l) (drop (S n) (Mem.stack m)) (tl (Mem.stack m')))
+   (*SACC:*)(IG: inject_globals ge j)
+   (*SACC:*)(*(INCR: inject_incr (Mem.flat_inj (Mem.nextblock init_m)) j)*)
+   (*SACC:*)(*(SEP: inject_separated (Mem.flat_inj (Mem.nextblock init_m)) j init_m init_m)*),
+      match_states (Returnstate s v m)
+                   (Returnstate s' v' m')
   | match_states_interm:
-      forall s sp pc rs m s' m' f r v' g j n l
-             (STACKS: match_stackframes j n g s s')
-             (MLD: Mem.inject j (S n :: g ++ l) m m')
-             (RETspec: is_return_spec f pc r)
-             (SZzero: f.(fn_stacksize) = 0)
-             (LDret: Val.inject j (rs#r) v')
-             (SZ: tc_sizes (g++l) (drop (S n) (Mem.stack m)) (tl (Mem.stack m')))
-             (IG: inject_globals ge j)
-             (INCR: inject_incr (Mem.flat_inj (Mem.nextblock init_m)) j)
-             (SEP: inject_separated (Mem.flat_inj (Mem.nextblock init_m)) j init_m init_m),
-        match_states (State s f (Vptr sp Ptrofs.zero) pc rs m)
-                     (Returnstate s' v' m').
-
-Definition mem_state (s: state) : mem :=
-  match s with
-    State _ _ _ _ _ m
-  | Callstate _ _ _ m _
-  | Returnstate _ _ m => m
-  end.
-
-(* Definition match_state_ge {F V} (g: Genv.t F V) (s: state) := *)
-(*   Ple (Genv.genv_next g) (Mem.nextblock (mem_state s)). *)
-
-Definition current_sp_state (s: state) : option (option (block * Z)) :=
-  match s with
-    State _ f (Vptr sp _) _ _ _ => Some (Some (sp, fn_stacksize f))
-  | State _ _ _ _ _ _ => None
-  | _ => Some None
-  end.
-
-Definition stackblocks_of_stackframe (sf: stackframe) : option (block * Z) :=
-  match sf with
-  | (Stackframe _ f (Vptr sp _) _ _) => Some (sp,fn_stacksize f)
-  | _ => None
-  end.
-
-Definition stackframes_state (s: state) : list stackframe :=
-  match s with
-    State stk _ _ _ _ _ 
-  | Callstate stk _ _ _ _
-  | Returnstate stk _ _ => stk
-  end.
-
-Definition stack_blocks_of_state (s: state) : list (option (block * Z)) :=
-  match current_sp_state s with
-    Some (Some x) => Some x :: map stackblocks_of_stackframe (stackframes_state s)
-  | Some None => map stackblocks_of_stackframe (stackframes_state s)
-  | None => None :: map stackblocks_of_stackframe (stackframes_state s)
-  end.
-
-Definition sp_valid (s : state) : Prop :=
-  Forall (fun bz => match bz with
-                   Some (b,z) => Mem.valid_block (mem_state s) b
-                 | None => True
-                 end) (stack_blocks_of_state s).
+      forall s sp pc rs m s' m' f r v' (*SACC:*)g (*SACC:*)j (*SACC:*)n (*SACC:*)l
+            (STACKS: match_stackframes (*SACC:*)j (*SACC:*)n (*SACC:*)g s s')
+   (*SACC:comments this*)(*(MLD: Mem.extends m m'),*)
+   (*SACC:*)(MLD: Mem.inject j (S n :: g ++ l) m m')
+      (RETspec: is_return_spec f pc r)
+      (RETspec: f.(fn_stacksize) = 0)
+   (*SACC:comments this*)(*Val.lessdef (rs#r) v'*)
+   (*SACC:*)(LDret: Val.inject j (rs#r) v')
+   (*SACC:*)(SZ: tc_sizes (g++l) (drop (S n) (Mem.stack m)) (tl (Mem.stack m')))
+   (*SACC:*)(IG: inject_globals ge j)
+   (*SACC:*)(*(INCR: inject_incr (Mem.flat_inj (Mem.nextblock init_m)) j)*)
+   (*SACC:*)(*(SEP: inject_separated (Mem.flat_inj (Mem.nextblock init_m)) j init_m init_m)*),
+      match_states (State s f (Vptr sp Ptrofs.zero) pc rs m)
+                   (Returnstate s' v' m').
 
 (** The last case of [match_states] corresponds to the execution
   of a move/nop/return sequence in the original code that was
@@ -564,7 +499,7 @@ Definition sp_valid (s : state) : Prop :=
 Definition measure (st: state) : nat :=
   match st with
   | State s f sp pc rs m => (List.length s * (niter + 2) + return_measure f.(fn_code) pc + 1)%nat
-  | Callstate s f args m sz => 0%nat
+  | Callstate s f args m => 0%nat
   | Returnstate s v m => (List.length s * (niter + 2))%nat
   end.
 
@@ -583,192 +518,17 @@ Ltac EliminatedInstr :=
 (** The proof of semantic preservation, then, is a simulation diagram
   of the ``option'' kind. *)
 
-
-Lemma regs_inject_regs:
-  forall j rs1 rs2, regs_inject j rs1 rs2 ->
-  forall rl, Val.inject_list j rs1##rl rs2##rl.
-Proof.
-  induction rl; constructor; auto.
-Qed.
-
-Lemma set_reg_inject:
-  forall j r v1 v2 rs1 rs2,
-  Val.inject j v1 v2 -> regs_inject j rs1 rs2 -> regs_inject j (rs1#r <- v1) (rs2#r <- v2).
-Proof.
-  intros; red; intros. repeat rewrite Regmap.gsspec.
-  destruct (peq r0 r); auto.
-Qed.
-
-Lemma set_res_inject:
-  forall j res v1 v2 rs1 rs2,
-  Val.inject j v1 v2 -> regs_inject j rs1 rs2 ->
-  regs_inject j (regmap_setres res v1 rs1) (regmap_setres res v2 rs2).
-Proof.
-  intros. destruct res; simpl; auto. apply set_reg_inject; auto.
-Qed.
-
-Lemma ros_is_function_transf:
-  forall j ros rs rs' id,
-    inject_globals ge j ->
-    ros_is_function ge ros rs id ->
-    regs_inject j rs rs' ->
-    ros_is_function tge ros rs' id.
-Proof.
-  unfold ros_is_function. intros.
-  destr_in H0. simpl.
-  destruct H0 as (b & o & RS & FS).
-  specialize (H1 r). rewrite RS in H1; inv H1.
-  eexists; eexists; split; eauto.
-  rewrite symbols_preserved. rewrite FS.
-  f_equal.
-  destruct H. erewrite H in H4. inv H4. auto. 
-  eapply Genv.genv_symb_range; eauto.
-Qed.
-
-Lemma inject_globals_meminj_preserves_globals:
-  forall {F V} (g: Genv.t F V) j,
-    inject_globals g j ->
-    meminj_preserves_globals g j.
-Proof.
-  intros F V g j (IG1 & IG2); split; [|split].
-  - intros id b FS.
-    eapply IG1. eapply Genv.genv_symb_range; eauto.
-  - intros b gv FVI.
-    unfold Genv.find_var_info in FVI.
-    repeat destr_in FVI.
-    eapply IG1. eapply Genv.genv_defs_range; eauto.
-  - intros b1 b2 delta gv FVI JB.
-    unfold Genv.find_var_info in FVI.
-    repeat destr_in FVI.
-    eapply IG2 in JB; eauto. apply JB. eapply Genv.genv_defs_range; eauto.
-Qed.
-
-
-Lemma regs_inject_init_regs:
-  forall j params vl vl',
-    Val.inject_list j vl vl' ->
-    regs_inject j (init_regs vl params) (init_regs vl' params).
-Proof.
-  induction params; intros.
-  simpl. red; intros. rewrite Regmap.gi. constructor.
-  simpl. inv H.   red; intros. rewrite Regmap.gi. constructor.
-  apply set_reg_inject. auto. auto.
-Qed.
-
-Lemma match_stackframes_incr:
-  forall f n l s s'
-    (MS: match_stackframes f n l s s')
-    f' (INCR: inject_incr f f'),
-    match_stackframes f' n l s s'.
-Proof.
-  induction 1; simpl; intros; eauto; try now econstructor; eauto.
-  econstructor; eauto.
-  red; intros; eauto.
-Qed.
-
-Lemma inject_globals_incr:
-  forall f f'
-    (INCR : inject_incr f f')
-    (SEP : forall b1 b2 delta, f b1 = None -> f' b1 = Some (b2, delta) -> Ple (Genv.genv_next ge) b1 /\ Ple (Genv.genv_next ge) b2)
-    (IG: inject_globals ge f),
-    inject_globals ge f'.
-Proof.
-  intros f f' INCR SEP (IG1 & IG2); split; intros; eauto.
-  eapply IG2; eauto.
-  destruct (f b1) eqn:FB1.
-  - destruct p. eapply INCR in FB1. congruence.
-  - specialize (SEP _ _ _ FB1 H).
-    xomega.
-Qed.
-
-
-Lemma tl_iter_commut:
-  forall {A} (l: list A) n,
-    tl (Nat.iter n (@tl _) l) = Nat.iter n (@tl _) (tl l).
-Proof.
-  induction n; simpl; intros; eauto. rewrite IHn. auto.
-Qed.
-
-Hypothesis init_m_genv_next:
-  Ple (Genv.genv_next ge) (Mem.nextblock init_m).
-
-Definition nextblock_inv (s: state) :=
-  Ple (Mem.nextblock init_m) (Mem.nextblock (mem_state s)).
-
-Lemma tc_sizes_same_top:
-  forall g f1 r1 f2 r2 f1' f2',
-    tc_sizes g (f1::r1) (f2::r2) ->
-    size_frames f1 = size_frames f1' ->
-    size_frames f2 = size_frames f2' ->
-    tc_sizes g (f1'::r1) (f2'::r2).
-Proof.
-  intros g f1 r1 f2 r2 f1' f2' SZ EQ1 EQ2.
-  inv SZ. simpl in *. repeat destr_in H4.
-  econstructor; simpl. eauto. rewrite Heqo. eauto.
-  rewrite <- EQ2.
-  inv H5; [left|right]. omega. auto.
-Qed.
-
-Lemma match_stackframes_no_perm':
-  forall j n g s s' P,
-    match_stackframes j n g s s' ->
-    forall stk sp,
-      stack_agree_perms P stk ->
-      match_stack (Some (sp, 0) :: map block_of_stackframe s) stk ->
-      forall l0,
-        take (S n) stk = Some l0 ->
-        Forall (fun tf => forall b, in_frames tf b -> forall o k p, ~ P b o k p) l0.
-Proof.
-  induction 1; simpl; intros stk0 sp0 SAP MS l0 TAKE; eauto.
-  - repeat destr_in TAKE.
-    constructor; auto. inv MS. unfold in_frames; simpl.
-    unfold get_frame_blocks; rewrite BLOCKS. simpl. intros b [[]|[]].
-    intros o k p PERM.
-    exploit SAP. left. reflexivity. simpl. reflexivity. rewrite BLOCKS; left; reflexivity.
-    eauto. rewrite SIZE. rewrite Z.max_id. omega.
-  - repeat destr_in TAKE.
-    constructor; auto. inv MS. unfold in_frames; simpl.
-    unfold get_frame_blocks; rewrite BLOCKS. simpl. intros b [[]|[]].
-    intros o k p PERM.
-    exploit SAP. left. reflexivity. simpl. reflexivity. rewrite BLOCKS; left; reflexivity.
-    eauto. rewrite SIZE. rewrite Z.max_id. omega.
-  - repeat destr_in TAKE. repeat destr_in Heqo.
-    constructor; eauto.
-    + inv MS. unfold in_frames; simpl.
-      unfold get_frame_blocks; rewrite BLOCKS. simpl. intros b [[]|[]].
-      intros o k p PERM.
-      exploit SAP. left. reflexivity. simpl. reflexivity. rewrite BLOCKS; left; reflexivity.
-      eauto. rewrite SIZE. rewrite Z.max_id. omega.
-    + inv MS. rewrite H1 in REC. eapply IHmatch_stackframes in REC; eauto.
-      eapply stack_agree_perms_tl in SAP; simpl in *; auto.
-      simpl. rewrite Heqo0. reflexivity.
-Qed.
-
-Lemma match_stackframes_no_perm:
-  forall j n g s s',
-    match_stackframes j n g s s' ->
-    forall m sp sz,
-      sz = 0 ->
-      match_stack (Some (sp, sz) :: map block_of_stackframe s) (Mem.stack m) ->
-      forall l0,
-        take (S n) (Mem.stack m) = Some l0 ->
-        Forall (fun tf => forall b, in_frames tf b -> forall o k p, ~ Mem.perm m b o k p) l0.
-Proof.
-  intros; subst; eapply match_stackframes_no_perm'; eauto.
-  apply Mem.agree_perms_mem. 
-Qed.
-
 Lemma transf_step_correct:
-  forall s1 t s2, step fn_stack_requirements ge s1 t s2 ->
-  forall s1' (MS: match_states s1 s1') (NI1: nextblock_inv s1) (NI2: nextblock_inv s1') (SPV: sp_valid s1) (* (MSA: match_stack s1) *) (MSA: stack_inv s1) (MSA': stack_inv s1'),
-  (exists s2', step fn_stack_requirements tge s1' t s2' /\ match_states s2 s2')
+  forall s1 t s2, step ge s1 t s2 ->
+  forall s1' (MS: match_states s1 s1'),
+  (exists s2', step tge s1' t s2' /\ match_states s2 s2')
   \/ (measure s2 < measure s1 /\ t = E0 /\ match_states s2 s1')%nat.
 Proof.
   induction 1; intros; inv MS; EliminatedInstr.
 
 - (* nop *)
   TransfInstr. left. econstructor; split.
-  eapply exec_Inop; eauto. econstructor; eauto.
+  eapply exec_Inop; eauto. constructor; auto.
 - (* eliminated nop *)
   assert (s0 = pc') by congruence. subst s0.
   right. split. simpl. omega. split. auto.
@@ -776,15 +536,13 @@ Proof.
 
 - (* op *)
   TransfInstr.
-  assert (Val.inject_list j (rs##args) (rs'##args)). apply regs_inject_regs; auto.
-  exploit eval_operation_inject; eauto.
-  eapply inject_globals_meminj_preserves_globals; eauto.
+  assert (Val.lessdef_list (rs##args) (rs'##args)). apply regs_lessdef_regs; auto.
+  exploit eval_operation_lessdef; eauto.
   intros [v' [EVAL' VLD]].
-  left. exists (State s' (transf_function f) (Vptr sp' Ptrofs.zero) pc' (rs'#res <- v') m'); split.
+  left. exists (State s' (transf_function f) (Vptr sp0 Ptrofs.zero) pc' (rs'#res <- v') m'); split.
   eapply exec_Iop; eauto.  rewrite <- EVAL'.
-  rewrite eval_shift_stack_operation.
   apply eval_operation_preserved. exact symbols_preserved.
-  econstructor; eauto. apply set_reg_inject; auto.
+  econstructor; eauto. apply set_reg_lessdef; auto.
 - (* eliminated move *)
   rewrite H1 in H. clear H1. inv H.
   right. split. simpl. omega. split. auto.
@@ -792,294 +550,135 @@ Proof.
 
 - (* load *)
   TransfInstr.
-  assert (Val.inject_list j (rs##args) (rs'##args)). apply regs_inject_regs; auto.
-  exploit eval_addressing_inject; eauto.
-  eapply inject_globals_meminj_preserves_globals; eauto.
+  assert (Val.lessdef_list (rs##args) (rs'##args)). apply regs_lessdef_regs; auto.
+  exploit eval_addressing_lessdef; eauto.
   intros [a' [ADDR' ALD]].
-  exploit Mem.loadv_inject; eauto.
+  exploit Mem.loadv_extends; eauto.
   intros [v' [LOAD' VLD]].
-  left. exists (State s' (transf_function f) (Vptr sp' Ptrofs.zero) pc' (rs'#dst <- v') m'); split.
-  eapply exec_Iload with (a0 := a'). eauto.  rewrite <- ADDR'.
-  rewrite eval_shift_stack_addressing.
+  left. exists (State s' (transf_function f) (Vptr sp0 Ptrofs.zero) pc' (rs'#dst <- v') m'); split.
+  eapply exec_Iload with (a := a'). eauto.  rewrite <- ADDR'.
   apply eval_addressing_preserved. exact symbols_preserved. eauto.
-  econstructor; eauto. apply set_reg_inject; auto.
+  econstructor; eauto. apply set_reg_lessdef; auto.
 
 - (* store *)
   TransfInstr.
-  assert (Val.inject_list j (rs##args) (rs'##args)). apply regs_inject_regs; auto.
-  exploit eval_addressing_inject; eauto.
-  eapply inject_globals_meminj_preserves_globals; eauto.
+  assert (Val.lessdef_list (rs##args) (rs'##args)). apply regs_lessdef_regs; auto.
+  exploit eval_addressing_lessdef; eauto.
   intros [a' [ADDR' ALD]].
-  exploit Mem.storev_mapped_inject. 2: eexact H1. eauto. eauto. apply RLD.
+  exploit Mem.storev_extends. 2: eexact H1. eauto. eauto. apply RLD.
   intros [m'1 [STORE' MLD']].
-  left. exists (State s' (transf_function f) (Vptr sp' Ptrofs.zero) pc' rs' m'1); split.
-  eapply exec_Istore with (a0 := a'). eauto.  rewrite <- ADDR'.
-  rewrite eval_shift_stack_addressing.
+  left. exists (State s' (transf_function f) (Vptr sp0 Ptrofs.zero) pc' rs' m'1); split.
+  eapply exec_Istore with (a := a'). eauto.  rewrite <- ADDR'.
   apply eval_addressing_preserved. exact symbols_preserved. eauto.
   destruct a; simpl in H1; try discriminate.
   econstructor; eauto.
-  repeat rewrite_stack_blocks; eauto.
 
 - (* call *)
   exploit find_function_translated; eauto. intro FIND'.
   TransfInstr.
 + (* call turned tailcall *)
-  assert (X: { m'' | Mem.free m' sp' 0 (fn_stacksize (transf_function f)) = Some m''}).
-  {
+  assert ({ m'' | Mem.free m' sp0 0 (fn_stacksize (transf_function f)) = Some m''}).
     apply Mem.range_perm_free. rewrite stacksize_preserved. rewrite H7.
     red; intros; omegaContradiction.
-  }
   destruct X as [m'' FREE].
-  generalize (Mem.free_right_inject _ _ _ _ _ _ _ _ MLD FREE). intro FINJ.
-  trim FINJ.
-  {
-    unfold Mem.flat_inj.
-    intros b1 delta ofs k p FI PERM RNG.
-    repeat destr_in FI.
-    rewrite stacksize_preserved in RNG. rewrite H7 in RNG. omega.
-  }
-  repeat rewrite_stack_blocks; eauto.
-
-  edestruct Mem.inject_new_stage_left_tailcall_right as (m2' & TCS & INJ'). apply FINJ.
-
-  eapply match_stackframes_no_perm; eauto.
-  inv MSA. eauto. 
-
-
-  inv MSA'. inv MSA1. eapply Mem.free_top_tframe_no_perm; eauto.
-
-  left. eexists (Callstate s' (transf_fundef fd) (rs'##args) m2' (fn_stack_requirements id)); split.
-  eapply exec_Itailcall; eauto.
-  eapply ros_is_function_transf; eauto.
-  apply sig_preserved.
-  econstructor. econstructor; eauto. all: auto.
-  apply regs_inject_regs; auto.
-  eauto.
-  repeat rewrite_stack_blocks. intro.
- 
-  eapply sizes_upstar'. rewrite <- EQ1. auto.
-
+  left. exists (Callstate s' (transf_fundef fd) (rs'##args) m''); split.
+  eapply exec_Itailcall; eauto. apply sig_preserved.
+  constructor. eapply match_stackframes_tail; eauto. apply regs_lessdef_regs; auto.
+  eapply Mem.free_right_extends; eauto.
+  rewrite stacksize_preserved. rewrite H7. intros. omegaContradiction.
 + (* call that remains a call *)
-  left. exists (Callstate (Stackframe res (transf_function f) (Vptr sp' Ptrofs.zero) pc' rs' :: s')
-                     (transf_fundef fd) (rs'##args) (Mem.push_new_stage m') (fn_stack_requirements id)); split.
-  eapply exec_Icall; eauto.
-  eapply ros_is_function_transf; eauto.
-  apply sig_preserved.
-  econstructor. constructor; eauto. all: auto.
-  apply regs_inject_regs; auto.
-  apply Mem.push_new_stage_inject. eauto.
-  repeat rewrite_stack_blocks. eapply tc_sizes_up; eauto.
+  left. exists (Callstate (Stackframe res (transf_function f) (Vptr sp0 Ptrofs.zero) pc' rs' :: s')
+                          (transf_fundef fd) (rs'##args) m'); split.
+  eapply exec_Icall; eauto. apply sig_preserved.
+  constructor. constructor; auto. apply regs_lessdef_regs; auto. auto.
 
 - (* tailcall *)
   exploit find_function_translated; eauto. intro FIND'.
-  exploit Mem.free_parallel_inject; eauto. constructor.
-  intros [m'1 [FREE EXT]].
-  destruct (Mem.tailcall_stage_inject _ _ _ _ _ EXT H3) as (m2' & TC & INJ).
-  {
-    inv MSA'. inv MSA1.
-    eapply Mem.free_top_tframe_no_perm; eauto.
-    rewrite stacksize_preserved in SIZE. rewrite Z.add_0_r. auto.
-  }
+  exploit Mem.free_parallel_extends; eauto. intros [m'1 [FREE EXT]].
   TransfInstr.
-  left. exists (Callstate s' (transf_fundef fd) (rs'##args) m2' (fn_stack_requirements id)); split.
-  eapply exec_Itailcall; eauto.
-  eapply ros_is_function_transf; eauto.
-  apply sig_preserved.
-  rewrite stacksize_preserved; auto. rewrite ! Z.add_0_r in FREE. eauto. auto.
-  econstructor; eauto.
-  apply regs_inject_regs; auto.
-  {
-    repeat rewrite_stack_blocks.
-    intros A B; rewrite A, B in SZ.
-    intros; eapply tc_sizes_same_top; eauto.
-    symmetry; apply size_frames_tc.
-    symmetry; apply size_frames_tc.
-  }
+  left. exists (Callstate s' (transf_fundef fd) (rs'##args) m'1); split.
+  eapply exec_Itailcall; eauto. apply sig_preserved.
+  rewrite stacksize_preserved; auto.
+  constructor. auto.  apply regs_lessdef_regs; auto. auto.
 
 - (* builtin *)
   TransfInstr.
-  exploit (@eval_builtin_args_inject _ _ _ _ ge tge (fun r => rs#r) (fun r => rs'#r) (Vptr sp0 Ptrofs.zero)); eauto.
-  {
-    simpl. intros; rewrite symbols_preserved; auto.
-  }
-  {
-    simpl; intros.
-    eapply IG; eauto. eapply Genv.genv_symb_range; eauto.
-  }
+  exploit (@eval_builtin_args_lessdef _ ge (fun r => rs#r) (fun r => rs'#r)); eauto.
   intros (vargs' & P & Q).
-  exploit external_call_mem_inject; eauto.
-  eapply inject_globals_meminj_preserves_globals; eauto.
-  apply Mem.push_new_stage_inject. eauto.
-  intros [f' [v' [m'1 [A [B [C [D [E [F G]]]]]]]]].
-  edestruct Mem.unrecord_stack_block_inject_parallel as (m'2 & USB & INJ'). apply C. eauto.
-  left. exists (State s' (transf_function f) (Vptr sp' Ptrofs.zero) pc' (regmap_setres res v' rs') m'2); split.
+  exploit external_call_mem_extends; eauto.
+  intros [v' [m'1 [A [B [C D]]]]].
+  left. exists (State s' (transf_function f) (Vptr sp0 Ptrofs.zero) pc' (regmap_setres res v' rs') m'1); split.
   eapply exec_Ibuiltin; eauto.
+  eapply eval_builtin_args_preserved with (ge1 := ge); eauto. exact symbols_preserved.
   eapply external_call_symbols_preserved; eauto. apply senv_preserved.
-  econstructor. 3: eauto.
-  all: eauto.
-  eapply match_stackframes_incr; eauto.
-  apply set_res_inject; auto.
-  red; intros; eauto.
-  repeat rewrite_stack_blocks. simpl. eauto.
-  eapply inject_globals_incr; eauto.
-  intros.
-  specialize (G _ _ _ H3 H4). unfold Mem.valid_block in G.
-  red in NI1. simpl in NI1.
-  red in NI2. simpl in NI2.
-  rewrite ! Mem.push_new_stage_nextblock in G.
-  xomega.
-  eapply inject_incr_trans; eauto.
-  {
-    red. intros b1 b2 delta F1 F2.
-    split.
-    unfold Mem.flat_inj in F1. now destr_in F1.
-    destruct (j b1) as [[b2' delta']|] eqn:JB1.
-    exploit F. apply JB1. rewrite F2; intro X; inv X.
-    eapply SEP; eauto.
-    exploit G. apply JB1. apply F2. unfold Mem.valid_block. rewnb. intros.
-    red in NI1, NI2. simpl in *. xomega.
-  }
-  
+  econstructor; eauto. apply set_res_lessdef; auto.
+
 - (* cond *)
   TransfInstr.
-  left. exists (State s' (transf_function f) (Vptr sp' Ptrofs.zero) (if b then ifso else ifnot) rs' m'); split.
+  left. exists (State s' (transf_function f) (Vptr sp0 Ptrofs.zero) (if b then ifso else ifnot) rs' m'); split.
   eapply exec_Icond; eauto.
-  eapply eval_condition_inject. apply regs_inject_regs; auto.
-  eauto. eauto. auto.
-  econstructor; eauto.
+  apply eval_condition_lessdef with (rs##args) m; auto. apply regs_lessdef_regs; auto.
+  constructor; auto.
 
 - (* jumptable *)
   TransfInstr.
-  left. exists (State s' (transf_function f) (Vptr sp' Ptrofs.zero) pc' rs' m'); split.
+  left. exists (State s' (transf_function f) (Vptr sp0 Ptrofs.zero) pc' rs' m'); split.
   eapply exec_Ijumptable; eauto.
   generalize (RLD arg). rewrite H0. intro. inv H2. auto.
-  econstructor; eauto.
+  constructor; auto.
 
 - (* return *)
-  exploit Mem.free_parallel_inject; eauto. constructor. intros [m'1 [FREE EXT]].
+  exploit Mem.free_parallel_extends; eauto. intros [m'1 [FREE EXT]].
   TransfInstr.
   left. exists (Returnstate s' (regmap_optget or Vundef rs') m'1); split.
-  eapply exec_Ireturn; eauto.
-  rewrite stacksize_preserved; auto. rewrite ! Z.add_0_r in FREE. eauto.
-  econstructor; eauto.
+  apply exec_Ireturn; auto. rewrite stacksize_preserved; auto.
+  constructor. auto.
   destruct or; simpl. apply RLD. constructor.
-  repeat rewrite_stack_blocks; eauto.
-  eapply tc_sizes_ndown; eauto.
-  
+  auto.
+
 - (* eliminated return None *)
   assert (or = None) by congruence. subst or.
   right. split. simpl. omega. split. auto.
-  econstructor. eauto. simpl. constructor.
-  eapply Mem.free_left_inject; eauto. eauto.
-  repeat rewrite_stack_blocks; eauto.
-  eauto. auto. auto.
+  constructor. auto.
+  simpl. constructor.
+  eapply Mem.free_left_extends; eauto.
 
 - (* eliminated return Some *)
   assert (or = Some r) by congruence. subst or.
   right. split. simpl. omega. split. auto.
-  econstructor. eauto.
+  constructor. auto.
   simpl. auto.
-  eapply Mem.free_left_inject; eauto. eauto.
-  repeat rewrite_stack_blocks; eauto.
-  auto. auto. auto.
+  eapply Mem.free_left_extends; eauto.
 
 - (* internal call *)
-  exploit Mem.alloc_parallel_inject; eauto.
-  + instantiate (1 := 0). omega.
-  + instantiate (1 := fn_stacksize f). omega.
-  + intros [f' [m'1 [b2 [ALLOC [INJ [INCR' [FEQ FOLD]]]]]]].
-    assert (EQ: fn_stacksize (transf_function f) = fn_stacksize f /\
-                fn_entrypoint (transf_function f) = fn_entrypoint f /\
-                fn_params (transf_function f) = fn_params f).
-    {
-      unfold transf_function. destruct (zeq (fn_stacksize f) 0); auto.
-    }
-    destruct EQ as [EQ1 [EQ2 EQ3]].
-
-
-
-  exploit Mem.record_push_inject_alloc. 4: apply INJ. 2: eauto. all: eauto.
-  inv MSA'. auto.
-    * eapply tc_sizes_ndown in SZ; eauto.
-      repeat rewrite_stack_blocks.
-      eapply tc_sizes_size_stack in SZ. etransitivity.
-      apply SZ. rewrite <- tl_drop. apply size_stack_drop.
-    * intros (m2' & RSB & UINJ).
-      left. econstructor; split.
-      -- simpl. eapply exec_function_internal; eauto. rewrite EQ1; eauto.
-         rewrite EQ1; eauto.
-      -- rewrite EQ2. rewrite EQ3. econstructor. 3: eauto.
-         all: eauto.
-         eapply match_stackframes_incr; eauto.
-         apply regs_inject_init_regs. auto.
-         eapply val_inject_list_incr; eauto.
-         repeat rewrite_stack_blocks; eauto.
-         intros A B; rewrite A, B in SZ.
-         {
-           eapply tc_sizes_same_top.
-           eapply tc_sizes_record; eauto.
-           rewrite ! size_frames_cons. reflexivity.
-           rewrite ! size_frames_cons. reflexivity.
-         }
-         eapply inject_globals_incr; eauto.
-         intros.
-         destruct (peq b1 stk). subst. rewrite FEQ in H2; inv H2.
-         red in NI1, NI2. simpl in NI1, NI2.
-         apply Mem.alloc_result in H. apply Mem.alloc_result in ALLOC. subst. xomega.
-         rewrite FOLD in H2. congruence. auto.
-         eapply inject_incr_trans; eauto.
-         {
-           red. intros b1 b0 delta F1 F2.
-           split.
-           unfold Mem.flat_inj in F1. now destr_in F1.
-           destruct (j b1) as [[b2' delta']|] eqn:JB1.
-           exploit INCR'. apply JB1. rewrite F2; intro X; inv X.
-           eapply SEP; eauto.
-           destruct (peq b1 stk). subst. rewrite FEQ in F2; inv F2.
-           apply Mem.alloc_result in ALLOC. subst. unfold Mem.valid_block.
-           red in NI2. simpl in NI2. xomega.
-           rewrite FOLD in F2 by auto. congruence.
-         }
+  exploit Mem.alloc_extends; eauto.
+    instantiate (1 := 0). omega.
+    instantiate (1 := fn_stacksize f). omega.
+  intros [m'1 [ALLOC EXT]].
+  assert (fn_stacksize (transf_function f) = fn_stacksize f /\
+          fn_entrypoint (transf_function f) = fn_entrypoint f /\
+          fn_params (transf_function f) = fn_params f).
+    unfold transf_function. destruct (zeq (fn_stacksize f) 0); auto.
+  destruct H0 as [EQ1 [EQ2 EQ3]].
+  left. econstructor; split.
+  simpl. eapply exec_function_internal; eauto. rewrite EQ1; eauto.
+  rewrite EQ2. rewrite EQ3. constructor; auto.
+  apply regs_lessdef_init_regs. auto.
 
 - (* external call *)
-  exploit external_call_mem_inject; eauto.
-  eapply inject_globals_meminj_preserves_globals; eauto.
-  intros [f' [res' [m2' [A [B [C [D [E [F G]]]]]]]]].
+  exploit external_call_mem_extends; eauto.
+  intros [res' [m2' [A [B [C D]]]]].
   left. exists (Returnstate s' res' m2'); split.
-  econstructor; eauto.
+  simpl. econstructor; eauto.
   eapply external_call_symbols_preserved; eauto. apply senv_preserved.
-  econstructor. 3: eauto.
-  all: eauto.
-  eapply match_stackframes_incr; eauto.
-  repeat rewrite_stack_blocks; eauto.
-  eapply tc_sizes_ndown; eauto.
-  eapply inject_globals_incr; eauto.
-  intros.
-  specialize (G _ _ _ H0 H1). unfold Mem.valid_block in G.
-  red in NI1, NI2; simpl in NI1, NI2. xomega.
-  eapply inject_incr_trans; eauto.
-  {
-    red. intros b1 b2 delta F1 F2.
-    split.
-    unfold Mem.flat_inj in F1. now destr_in F1.
-    destruct (j b1) as [[b2' delta']|] eqn:JB1.
-    exploit F. apply JB1. rewrite F2; intro X; inv X.
-    eapply SEP; eauto.
-    exploit G. apply JB1. apply F2. unfold Mem.valid_block. rewnb. intros.
-    red in NI1, NI2. simpl in *. xomega.
-  }
+  constructor; auto.
 
 - (* returnstate *)
-  inv MS0.
+  inv H2.
 + (* synchronous return in both programs *)
-  left.
-  edestruct Mem.unrecord_stack_block_inject_parallel as (m'2 & USB & INJ'); eauto.
-  econstructor; split.
-  apply exec_return; eauto.
-  econstructor; eauto. apply set_reg_inject; auto.
-  repeat rewrite_stack_blocks.
-  simpl in *. auto.
-
+  left. econstructor; split.
+  apply exec_return.
+  constructor; auto. apply set_reg_lessdef; auto.
 + (* return instr in source program, eliminated because of tailcall *)
   right. split. unfold measure. simpl length.
   change (S (length s) * (niter + 2))%nat
@@ -1087,173 +686,43 @@ Proof.
   generalize (return_measure_bounds (fn_code f) pc). omega.
   split. auto.
   econstructor; eauto.
-  eapply Mem.unrecord_stack_block_inject_left. eauto. eauto.
-  omega.
-  inv MSA. auto.
   rewrite Regmap.gss. auto.
-  rewrite_stack_blocks. simpl in *.
-  auto.
 Qed.
-
-Lemma nextblock_inv_step:
-  forall ge s1 t s1'
-    (MSG: nextblock_inv s1)
-    (STEP: step fn_stack_requirements ge s1 t s1'),
-    nextblock_inv s1'.
-Proof.
-  intros ge0 s1 t s1' MSG STEP.
-  inv STEP; red in MSG; red; simpl in *; rewnb; auto.
-  xomega.
-Qed.
-
-Lemma sp_valid_step:
-  forall s1 t s1',
-    sp_valid s1 ->
-    step fn_stack_requirements ge s1 t s1' ->
-    sp_valid s1'.
-Proof.
-  intros s1 t s1' SPV STEP.
-  red in SPV; red.
-  unfold stack_blocks_of_state in *.
-  assert (valid_impl: forall b, Mem.valid_block (mem_state s1) b -> Mem.valid_block (mem_state s1') b).
-  {
-    inv STEP; simpl in *; intros; red; auto.
-    - red; erewrite Mem.storev_nextblock; eauto.
-    - rewrite Mem.push_new_stage_nextblock. auto.
-    - erewrite Mem.tailcall_stage_nextblock by eauto. erewrite Mem.nextblock_free; eauto.
-    - apply external_call_nextblock in H1. red in H3.
-      erewrite Mem.unrecord_stack_block_nextblock by eauto.
-      rewrite Mem.push_new_stage_nextblock in H1.
-      xomega.
-    - erewrite Mem.nextblock_free; eauto.
-    - erewrite Mem.record_stack_block_nextblock by eauto.
-      erewrite Mem.nextblock_alloc; eauto.
-      red in H1. xomega.
-    - apply external_call_nextblock in H. red in H0; xomega.
-    - erewrite Mem.unrecord_stack_block_nextblock; eauto.
-  }
-
-  assert (SPV': Forall
-          (fun bz : option (block * Z) =>
-           match bz with
-           | Some (b, _) => Mem.valid_block (mem_state s1') b
-           | None => True
-           end) match current_sp_state s1 with
-          | Some (Some x) => Some x :: map stackblocks_of_stackframe (stackframes_state s1)
-          | Some None => map stackblocks_of_stackframe (stackframes_state s1)
-          | None => None :: map stackblocks_of_stackframe (stackframes_state s1)
-          end).
-  {
-    eapply Forall_impl. 2: eauto. simpl; intros.
-    destr_in H0. destr. eauto.
-  }
-  inv STEP; simpl in *; intros; eauto.
-  - constructor; auto. destr. destr. destr_in Heqo. inv Heqo. inv SPV'; auto.
-    repeat destr_in SPV; inv SPV'; auto.
-  - inv SPV'; auto.
-  - inv SPV'; auto.
-  - constructor; auto. red; erewrite Mem.record_stack_block_nextblock by eauto.
-    eapply Mem.valid_new_block; eauto.
-  - inv SPV'; auto.
-    repeat destr; constructor; auto.
-    destr. destr_in Heqo.
-Qed.
-
-Definition match_states' s1 s2 :=
-  match_states s1 s2 /\ stack_inv s1 /\ stack_inv s2 /\
-  sp_valid s1 /\ nextblock_inv s1 /\ nextblock_inv s2.
-
-Hint Resolve nextblock_inv_step sp_valid_step stack_inv_inv.
-
-Lemma transf_step_correct':
-  forall s1 t s2,
-    step fn_stack_requirements ge s1 t s2 ->
-    forall s1',
-      match_states' s1 s1' ->
-      (exists s2', step fn_stack_requirements tge s1' t s2' /\ match_states' s2 s2') \/
-      (measure s2 < measure s1)%nat /\ t = E0 /\ match_states' s2 s1'.
-Proof.
-  intros s1 t s2 STEP s1' MS.
-  destruct MS as (MS & MSA & MSA' & SPV & MSG & MSG').
-  edestruct (transf_step_correct _ _ _ STEP _ MS) as
-      [(s2' & STEP' & MS')|(MLT & TE0 & MS')]; eauto.
-  - left. eexists; split; eauto.
-    repeat split; eauto.
-  - right; repeat split; eauto.
-Qed.
-
-End WITHINITMEM.
-
-Inductive ms (s1 s2 : state) : Prop :=
-| ms_intro init_m (INIT: Genv.init_mem prog = Some init_m) (MS: match_states' init_m s1 s2).
 
 Lemma transf_initial_states:
-  forall st1, initial_state fn_stack_requirements prog st1 ->
-  exists st2, initial_state fn_stack_requirements tprog st2 /\ ms st1 st2.
+  forall st1, initial_state prog st1 ->
+  exists st2, initial_state tprog st2 /\ match_states st1 st2.
 Proof.
   intros. inv H.
   exploit funct_ptr_translated; eauto. intro FIND.
-  exists (Callstate nil (transf_fundef f) nil (Mem.push_new_stage m2) (fn_stack_requirements (prog_main tprog))); split.
+  exists (Callstate nil (transf_fundef f) nil m0); split.
   econstructor; eauto. apply (Genv.init_mem_transf TRANSL). auto.
   replace (prog_main tprog) with (prog_main prog).
   rewrite symbols_preserved. eauto.
   symmetry; eapply match_program_main; eauto. 
   rewrite <- H3. apply sig_preserved.
-  erewrite <- match_program_main; eauto.
-  edestruct (Mem.record_init_sp_flat_inject m0 m0 m2) as (m2' & RIS & INJ); eauto.
-  eapply Genv.initmem_inject; eauto. omega. 
-  assert (m2 = m2') by congruence. subst.
-  econstructor. eauto.
-  split.
-  econstructor. constructor. constructor.
-  * apply Mem.push_new_stage_inject; eauto.
-  * repeat rewrite_stack_blocks. simpl.
-    repeat econstructor; omega.
-  * unfold Mem.flat_inj; rewnb.
-    fold ge. split; intros.
-    apply pred_dec_true; xomega.
-    destr_in H.
-  * red; intros. revert H; unfold Mem.flat_inj; rewnb.
-    repeat destr. exfalso; xomega.
-  * unfold Mem.flat_inj. red. unfold Mem.valid_block. rewnb. intros.
-    destr_in H. destr_in H5.
-  * repeat split.
-    -- red in TRANSL. apply match_program_main in TRANSL. rewrite TRANSL.
-       eapply stack_inv_initial. econstructor; eauto.
-    -- eapply stack_inv_initial. econstructor; eauto.
-       red in TRANSL.
-       eapply Genv.init_mem_transf in TRANSL; eauto.
-       erewrite (Genv.find_symbol_transf TRANSL). fold ge0.
-       red in TRANSL. apply match_program_main in TRANSL. rewrite TRANSL.
-       eauto.
-       rewrite sig_preserved; auto.
-    -- red; simpl. constructor.
-    -- red. simpl. rewnb. xomega.
-    -- red. simpl. rewnb. xomega.
+  constructor. constructor. constructor. apply Mem.extends_refl.
 Qed.
 
 Lemma transf_final_states:
   forall st1 st2 r,
-    ms st1 st2 -> final_state st1 r -> final_state st2 r.
+  match_states st1 st2 -> final_state st1 r -> final_state st2 r.
 Proof.
-  intros st1 st2 r MS FS. inv FS. inv MS. inv MS0. inv H. inv LDret. inv MS. constructor.
+  intros. inv H0. inv H. inv H5. inv H3. constructor.
 Qed.
+
 
 (** The preservation of the observable behavior of the program then
   follows. *)
 
 Theorem transf_program_correct:
-  forward_simulation (RTL.semantics fn_stack_requirements prog) (RTL.semantics fn_stack_requirements tprog).
+  forward_simulation (RTL.semantics prog) (RTL.semantics tprog).
 Proof.
   eapply forward_simulation_opt with (measure := measure); eauto.
   apply senv_preserved. 
   eexact transf_initial_states.
   eexact transf_final_states.
-  simpl. intros s1 t s1' STEP s2 MS. inv MS.
-  edestruct transf_step_correct' as [(s2' & STEP' & MS')|(LT & EMPTY & MS')]; eauto.
-  erewrite <- Genv.init_mem_genv_next; eauto. fold ge. xomega.
-  left; eexists; split; eauto. econstructor; eauto.
-  right; split; eauto. split; auto. econstructor; eauto.
+  exact transf_step_correct.
 Qed.
 
 End PRESERVATION.
